Use stack_limit + size Mptr as the size of the stack for RawAsm and RealAsm

x86/Asmexpand.ml
@@ -480,8 +480,6 @@ let set_al sg =
 
 let expand_instruction instr =
   match instr with
-  (instr,isz) ->
-  match instr with
   | Pallocframe (f, ofs_ra) ->
 let sz = StackADT.frame_size f in
      if Archi.ptr64 then begin
